src/tls13formats/handshake_data.rs
@@ -1,5 +1,5 @@
 use crate::tls13utils::{
-    bytes1, check_eq, encode_length_u24, eq1, length_u24_encoded, parse_failed, tlserr, Bytes,
+    check_eq1, encode_length_u24, eq1, length_u24_encoded, parse_failed, tlserr, Bytes,
     TLSError, U8,
 };
 
@@ -55,6 +55,7 @@ pub fn get_hs_type(t: u8) -> Result<HandshakeType, TLSError> {
 /// Hadshake data of the TLS handshake.
 pub struct HandshakeData(pub(crate) Bytes);
 
+#[hax_lib::attributes]
 impl HandshakeData {
     /// Generate a new [`HandshakeData`] from [`Bytes`] and the [`HandshakeType`].
     pub(crate) fn from_bytes(
@@ -98,16 +99,15 @@ impl HandshakeData {
         expected_type: HandshakeType,
     ) -> Result<HandshakeData, TLSError> {
         let (message, payload_rest) = self.next_handshake_message()?;
-        let HandshakeData(tagged_message_bytes) = if payload_rest.len() != 0 {
+        if payload_rest.len() != 0 {
             tlserr(parse_failed())
         } else {
-            Ok(message)
-        }?;
-        let expected_bytes = bytes1(expected_type as u8);
-        check_eq(&expected_bytes, &tagged_message_bytes.slice_range(0..1))?;
-        Ok(HandshakeData(
-            tagged_message_bytes.slice_range(4..tagged_message_bytes.len()),
-        ))
+            let HandshakeData(tagged_message_bytes) = message;
+            check_eq1(expected_type as u8, tagged_message_bytes[0])?;
+            Ok(HandshakeData(
+                tagged_message_bytes.slice_range(4..tagged_message_bytes.len()),
+            ))
+        }
     }
 
     /// Attempt to parse a handshake message from the beginning of the payload.
@@ -116,6 +116,9 @@ impl HandshakeData {
     /// payload. Returns a [TLSError] if the payload is too short to contain a
     /// handshake message or if the payload is shorter than the expected length
     /// encoded in its first three bytes.
+    #[hax_lib::ensures(|result| match result {
+                                        Result::Ok((m,_)) => m.len() >= 4,
+                                        _ => true })]
     pub(crate) fn next_handshake_message(&self) -> Result<(Self, Self), TLSError> {
         if (self.len()) < 4 {
             tlserr(parse_failed())
@@ -167,12 +170,13 @@ impl HandshakeData {
     /// Beginning at offset `start`, attempt to find a message of type `handshake_type` in `payload`.
     ///
     /// Returns `true`` if `payload` contains a message of the given type, `false` otherwise.
+    #[hax_lib::requires(fstar!(r#"Seq.length self._0._0 >= v start"#))]
     pub(crate) fn find_handshake_message(
         &self,
         handshake_type: HandshakeType,
         start: usize,
     ) -> bool {
-        if (self.len()) < start + 4 {
+        if self.len() - start < 4 {
             false
         } else {
             match length_u24_encoded(self.0.raw_slice(start + 1..self.0.len())) {
