proofs/fstar/extraction/Bertie.Tls13cert.fsti
@@ -30,13 +30,35 @@ val check_success (v_val: bool)
 
 /// Check that the tag has a certain value.
 val check_tag (b: Bertie.Tls13utils.t_Bytes) (offset: usize) (value: u8)
-    : Prims.Pure (Core.Result.t_Result Prims.unit u8) Prims.l_True (fun _ -> Prims.l_True)
+    : Prims.Pure (Core.Result.t_Result Prims.unit u8)
+      Prims.l_True
+      (ensures
+        fun result ->
+          let result:Core.Result.t_Result Prims.unit u8 = result in
+          match result <: Core.Result.t_Result Prims.unit u8 with
+          | Core.Result.Result_Ok _ -> (Bertie.Tls13utils.impl__Bytes__len b <: usize) >. offset
+          | _ -> true)
 
 val length_length (b: Bertie.Tls13utils.t_Bytes) (offset: usize)
-    : Prims.Pure usize Prims.l_True (fun _ -> Prims.l_True)
+    : Prims.Pure (Core.Result.t_Result usize u8)
+      Prims.l_True
+      (ensures
+        fun result ->
+          let result:Core.Result.t_Result usize u8 = result in
+          match result <: Core.Result.t_Result usize u8 with
+          | Core.Result.Result_Ok l ->
+            (Bertie.Tls13utils.impl__Bytes__len b <: usize) >. offset && l <=. sz 255
+          | _ -> true)
 
 val short_length (b: Bertie.Tls13utils.t_Bytes) (offset: usize)
-    : Prims.Pure (Core.Result.t_Result usize u8) Prims.l_True (fun _ -> Prims.l_True)
+    : Prims.Pure (Core.Result.t_Result usize u8)
+      Prims.l_True
+      (ensures
+        fun result ->
+          let result:Core.Result.t_Result usize u8 = result in
+          match result <: Core.Result.t_Result usize u8 with
+          | Core.Result.Result_Ok _ -> (Bertie.Tls13utils.impl__Bytes__len b <: usize) >. offset
+          | _ -> true)
 
 [@@ FStar.Tactics.Typeclasses.tcinstance]
 val impl:Core.Clone.t_Clone t_CertificateKey
@@ -47,7 +69,7 @@ val impl_1:Core.Marker.t_Copy t_CertificateKey
 /// Read the EC PK from the cert as uncompressed point.
 val ecdsa_public_key (cert: Bertie.Tls13utils.t_Bytes) (indices: t_CertificateKey)
     : Prims.Pure (Core.Result.t_Result Bertie.Tls13utils.t_Bytes u8)
-      Prims.l_True
+      (requires v indices._1 > 0 && Seq.length cert._0 >= v indices._0 + v indices._1)
       (fun _ -> Prims.l_True)
 
 /// Read an octet string from the provided bytes.
@@ -68,14 +90,30 @@ val read_version_number (b: Bertie.Tls13utils.t_Bytes) (offset: usize)
     : Prims.Pure (Core.Result.t_Result usize u8) Prims.l_True (fun _ -> Prims.l_True)
 
 val long_length (b: Bertie.Tls13utils.t_Bytes) (offset len: usize)
-    : Prims.Pure (Core.Result.t_Result usize u8) Prims.l_True (fun _ -> Prims.l_True)
+    : Prims.Pure (Core.Result.t_Result usize u8)
+      Prims.l_True
+      (ensures
+        fun result ->
+          let result:Core.Result.t_Result usize u8 = result in
+          match result <: Core.Result.t_Result usize u8 with
+          | Core.Result.Result_Ok _ ->
+            (Bertie.Tls13utils.impl__Bytes__len b <: usize) >=. offset &&
+            ((Bertie.Tls13utils.impl__Bytes__len b <: usize) -! offset <: usize) >=. len
+          | _ -> true)
 
 /// Get the length of an ASN.1 type.
 /// This assumes that the length starts at the beginning of the provided byte
 /// sequence.
 /// Returns: (offset, length)
 val length (b: Bertie.Tls13utils.t_Bytes) (offset: usize)
-    : Prims.Pure (Core.Result.t_Result (usize & usize) u8) Prims.l_True (fun _ -> Prims.l_True)
+    : Prims.Pure (Core.Result.t_Result (usize & usize) u8)
+      Prims.l_True
+      (ensures
+        fun result ->
+          let result:Core.Result.t_Result (usize & usize) u8 = result in
+          match result <: Core.Result.t_Result (usize & usize) u8 with
+          | Core.Result.Result_Ok _ -> (Bertie.Tls13utils.impl__Bytes__len b <: usize) >. offset
+          | _ -> true)
 
 /// Read an integer and return a copy of the actual bytes.
 val read_integer (b: Bertie.Tls13utils.t_Bytes) (offset: usize)
